### Example Calculation:

Letâ€™s calculate a few values manually to see how this works:

1. \( n = 1 \):
   $$\[
   S(1) = 1.
   \]$$
2. \( n = 2 \):
   \[
   S(2) = (S(1) + 2) \mod 2 = (1 + 2) \mod 2 = 1.
   \]
3. \( n = 3 \):
   \[
   $$
\begin{align}
   S(3) = (S(2) + 2) \mod 3 = (1 + 2) \mod 3 = 0 \Rightarrow S(3) = 3.
\end{align}
   $$
   \]
5. \( n = 4 \):
   \[
   S(4) = (S(3) + 2) \mod 4 = (3 + 2) \mod 4 = 1.
   \]
6. \( n = 5 \):
   \[
   S(5) = (S(4) + 2) \mod 5 = (1 + 2) \mod 5 = 3.
   \]
   
